removed mentions of Even and Odd models from spec proofs

fairis/heap_lang/examples/even_odd/eo_vs_mod.v
@@ -6,7 +6,7 @@ From iris.base_logic.lib Require Import invariants.
 From iris.proofmode Require Import tactics.
 From trillium.prelude Require Export finitary quantifiers sigma classical_instances.
 From trillium.program_logic Require Export weakestpre.
-From trillium.fairness Require Import fairness fair_termination utils action_model resources.
+From trillium.fairness Require Import fairness fair_termination utils action_model resources fuel.
 From trillium.fairness.heap_lang Require Export lang lifting tactics proofmode.
 From trillium.fairness.heap_lang Require Import notation sswp_rules iris_inst.
 From trillium.fairness.heap_lang.examples Require Import env_am split_model.
@@ -29,18 +29,8 @@ Class evenoddG (Σ: gFunctors) := EvenoddG {
 
 
 Section proof_start.
-  Context {even_impl: EvenModel} {odd_impl: OddModel}.
-  Context `(ENV_AM: EnvironmentAM env_AM).
-
-  Let PM := @prod_model even_impl odd_impl.
-  Context {prod_AM_act_dec: ∀ a, Decision (is_action_of PM a)}.
-
-  Let M := @the_fair_model even_impl odd_impl prod_AM_act_dec _ ENV_AM.
-  Let LM := @the_model even_impl odd_impl prod_AM_act_dec _ ENV_AM.
-
-  Hypothesis PROD_ENV_INDEP: forall a, is_action_of PM a -> is_action_of env_AM a -> False.
-
-  Context `{hGS: !heapGS Σ LM, !evenoddG Σ, SplitGS Σ PM env_AM}.
+  Context `{LM: LiveModel heap_lang M}. 
+  Context `{hGS: !heapGS Σ LM, !evenoddG Σ}.
 
   Context (st_res even_at odd_at: nat -> iProp Σ). 
   Context
@@ -48,15 +38,21 @@ Section proof_start.
     (st_res_SR_odd: @StateRes _ Nat.odd st_res odd_at). 
 
   Definition Ns__eo := nroot .@ "even_odd".
-  Definition Ns__split := nroot .@ "split".
-  Definition evenodd_inv n := inv Ns__eo (evenodd_inv_inner ENV_AM st_res n).
 
-  Let ρEven: fmrole M := inl $ even_role (ρ__e even_impl).
-  Let ρOdd: fmrole M := inl $ odd_role (ρ__o odd_impl).
+  Definition main_corr l (N: nat): iProp Σ :=
+    l ↦ #N ∗ st_res N.
+
+  Definition main_vs l ι: iProp Σ :=
+    □ |={⊤, ⊤ ∖ ↑ι}=> ∃ N,
+    ▷ main_corr l N ∗ (▷ main_corr l N ={⊤ ∖ ↑ι, ⊤}=∗ True). 
 
   Definition even_odd_spec (prog: val): Prop :=
-    forall tid n N1 N2 f (Hf: f > 60) (EVEN: N1 < N2), 
-    {{{ split_inv Ns__split ∗ evenodd_inv n ∗ 
+    forall tid n N1 N2 f (Hf: f > 60) (EVEN: N1 < N2) (ρEven ρOdd: fmrole M)
+    (NEQ: ρEven ≠ ρOdd)
+    (FUEL_LB: lm_flm LM ≥ 61),
+    {{{ even_vs st_res_SR_even n Ns__eo ρEven ∗
+        odd_vs st_res_SR_odd n Ns__eo ρOdd ∗
+        main_vs n Ns__eo ∗
         tid ↦M {[ ρEven := f; ρOdd := f ]} ∗
         even_at N1 ∗ odd_at N2 ∗ frag_free_roles_are ∅ }}}
       prog #n @ tid
@@ -70,29 +66,30 @@ Section proof_start.
       (Fork ((e_prog ep) "l" "x") ;;
        Fork ((o_prog op) "l" ("x"+#1))).
 
-  Existing Instance even_AME. 
-  Existing Instance odd_AME.
-
   Lemma start_spec: even_odd_spec start. 
   Proof using All.
-    rewrite /even_odd_spec. iIntros (tid n N1 N2 f Hf EVEN). 
-    iIntros (Φ) "(#SPLIT & #Hinv & Hf & Heven_at & Hodd_at & HFR) HΦ". unfold start.
+    rewrite /even_odd_spec. iIntros (tid n N1 N2 f Hf EVEN ρEven ρOdd ? ?).
+    iIntros (Φ) "(VS_E & VS_O & #VS_M & Hf & Heven_at & Hodd_at & HFR) HΦ".
+    unfold start.
     rewrite <- (union_empty_l_L ∅). 
     wp_pures.
     wp_bind (Load _).
     iApply wp_atomic.
-    iInv Ns__eo as (m) "(>CUR & >Hn & Hauths)" "Hclose".
+
+    rewrite /main_vs.
+    iPoseProof "VS_M" as "-#V". iMod "V" as (m) "((Hn & Hauths) & Clos)". 
+    (* iInv Ns__eo as (m) "(>CUR & >Hn & Hauths)" "Hclose". *)
     iIntros "!>". wp_load. iIntros "!>".
     
     iDestruct (sr_agree _ _ _ st_res_SR_even with "[$] [$]") as %->.
     iDestruct (sr_agree _ _ _ st_res_SR_odd with "[$] [$]") as %->.
-    rewrite -Nat.negb_even in EVEN. destruct (Nat.even m) eqn:E; simpl in EVEN; [| lia].
+    rewrite -Nat.negb_even in EVEN. destruct (Nat.even m) eqn:E; simpl in EVEN; [| lia].    
 
-    iMod ("Hclose" with "[-Hf Heven_at Hodd_at HΦ]") as "_".
-    { iIntros "!>". iExists _. iFrame. }
+    iMod ("Clos" with "[Hn Hauths]") as "_"; [by iFrame| ]. 
+
     iIntros "!>". wp_pures. wp_bind (Fork _).
     iApply (wp_role_fork _ tid _ _ _ {[ρOdd := _]} {[ρEven := _]}
-             with "[Hf ] [Heven_at]"). 
+             with "[Hf ] [Heven_at VS_E]"). 
     { apply map_disjoint_dom. rewrite !dom_singleton.
       destruct (Nat.even m); set_solver. }
     { intros Hempty%map_positive_l. set_solver. }
@@ -104,14 +101,13 @@ Section proof_start.
       rewrite map_disjoint_dom. set_solver. }
     { iIntros (tid') "!> Hf".
       iApply (@e_spec ep M _ _ _ _ _ st_res_SR_even
-               with "[$Hf $Heven_at]"); [lia| simpl; lia | ..].
-      2: { by iIntros "!> ?". }
-      iApply even_vs; eauto. solve_ndisj. }
+               with "[$Hf $Heven_at $VS_E]"); [lia| simpl; lia | ..].
+      by iIntros "!> ?". }
 
     iIntros "!> Hf".
     iIntros "!>".
     wp_pures.
-    iApply (wp_role_fork _ tid _ _ _ ∅ _ with "[Hf] [Hodd_at]").
+    iApply (wp_role_fork _ tid _ _ _ ∅ _ with "[Hf] [Hodd_at VS_O]").
     { apply map_disjoint_dom. apply map_disjoint_dom. apply map_disjoint_empty_l. }
     2: { rewrite has_fuels_gt_1; last solve_fuel_positive.
          rewrite !fmap_insert fmap_empty //.
@@ -124,29 +120,18 @@ Section proof_start.
       replace (Z.of_nat m + 1)%Z with (Z.of_nat (m + 1)) by lia.
       rewrite -Nat.negb_even E. 
       iApply (@o_spec op M _ _ _ _ _ st_res_SR_odd
-               with "[$Hf $Hodd_at]"); [lia| simpl; lia | ..].
-      2: { by iIntros "!> ?". }
-      iApply odd_vs; eauto. solve_ndisj. }
+               with "[$Hf $Hodd_at $VS_O]"); [lia| simpl; lia | ..].
+      by iIntros "!> ?". }
 
     iIntros "!> Hf". by iApply "HΦ". 
-  Qed. 
+   Qed. 
 
 End proof_start.
 
 
 Section short_prog.
-  Context {even_impl: EvenModel} {odd_impl: OddModel}.
-  Context `(ENV_AM: EnvironmentAM env_AM).
-
-  Let PM := @prod_model even_impl odd_impl.
-  Context {prod_AM_act_dec: ∀ a, Decision (is_action_of PM a)}. 
-
-  Let M := @the_fair_model even_impl odd_impl prod_AM_act_dec _ ENV_AM.
-  Let LM := @the_model even_impl odd_impl prod_AM_act_dec _ ENV_AM.
-
-  Hypothesis PROD_ENV_INDEP: forall a, is_action_of PM a -> is_action_of env_AM a -> False.
-
-  Context `{hGS: !heapGS Σ LM, !evenoddG Σ, SplitGS Σ PM env_AM}.
+  Context `{LM: LiveModel heap_lang M}. 
+  Context `{hGS: !heapGS Σ LM, !evenoddG Σ}.
 
   Context (st_res even_at odd_at: nat -> iProp Σ). 
   Context
@@ -159,25 +144,26 @@ Section short_prog.
       "short" "l"
   .
   
-  Let ρEven: fmrole M := inl $ even_role (ρ__e even_impl).
-  Let ρOdd: fmrole M := inl $ odd_role (ρ__o odd_impl).
-
   Lemma sub_helper: forall y, y >= 1 -> S (y - 1) = y.
   Proof. lia. Qed. 
 
   Lemma add_helper: forall y d, y >= d -> (y - d) + d = y.
   Proof. lia. Qed.
 
-  (* Definition Ns := nroot .@ "eo". *)
-  (* Definition split_inv: iProp Σ := inv Ns (split_inv_inner (hGS := hGS)). *)
-
   Lemma short_spec_impl tid n N1 N2 
     (ev := Nat.ltb N1 N2)
     (d := 10)
     (b := 40)
+    (ρEven ρOdd: fmrole M)
+    (NEQ: ρEven ≠ ρOdd)
     f1 f2 (Hf1: f1 > b) (Hf2: f2 > b)
+    (FUEL_LB: lm_flm LM ≥ 61)
     :
-    {{{ split_inv Ns__split ∗ evenodd_inv ENV_AM st_res n ∗ 
+    {{{ 
+        (* split_inv Ns__split ∗ evenodd_inv ENV_AM st_res n ∗  *)
+         even_vs st_res_SR_even n Ns__eo ρEven ∗
+        odd_vs st_res_SR_odd n Ns__eo ρOdd ∗
+        main_vs st_res n Ns__eo ∗
         tid ↦M {[ ρEven := f1 + (if ev then 0 else d); ρOdd := f2 + (if ev then d else 0) ]} ∗
         even_at N1 ∗ odd_at N2 ∗ frag_free_roles_are ∅
     }}}
@@ -186,17 +172,19 @@ Section short_prog.
   Proof using All.
     subst ev. 
     iLöb as "Hg" forall (N1 N2 f1 Hf1 f2 Hf2).
-    iIntros (Φ) "(#SPLIT & #Hinv & Hf & Heven_at & Hodd_at & HFR) HΦ". 
+    iIntros (Φ) "(#VS_E & #VS_O & #VS_M & Hf & Heven_at & Hodd_at & HFR) HΦ".
     rewrite /short.
 
     wp_lam.
     wp_bind (!_)%E. iApply wp_atomic.
-    iInv Ns__eo as (m) "(>CUR & >Hn & Hauths)" "Hclose".
+    (* iInv Ns__eo as (m) "(>CUR & >Hn & Hauths)" "Hclose". *)
+    iPoseProof "VS_M" as "-#V". iMod "V" as (m) "((Hn & Hauths) & Clos)". 
+
     iIntros "!>". wp_load. iIntros "!>".
     iDestruct (sr_agree _ _ _ st_res_SR_even with "[$] [$]") as %->.
     iDestruct (sr_agree _ _ _ st_res_SR_odd with "[$] [$]") as %->.
     rewrite -Nat.negb_even.
-    iMod ("Hclose" with "[Hauths CUR Hn]") as "_".
+    iMod ("Clos" with "[Hauths Hn]") as "_".
     { iFrame. }
     iModIntro.
 
@@ -205,19 +193,20 @@ Section short_prog.
 
     destruct (Nat.even m) eqn:E; simpl.  
     - erewrite (proj2 (Nat.ltb_lt _ _)); [| lia].
-      iPoseProof (even_vs  _ _ _ _ st_res_SR_even with "[$]") as "#VS".
-      { solve_ndisj. }
-      rewrite /eo_vs. iMod "VS".
-      iDestruct "VS" as (m') "[CORR MU]".
+      (* iPoseProof (even_vs  _ _ _ _ st_res_SR_even with "[$]") as "#VS". *)
+      (* { solve_ndisj. } *)
+      (* rewrite /eo_vs. *)
+      (* iDestruct "VS" as (m') "[CORR MU]". *)
+      iPoseProof "VS_E" as "-#V". iMod "V" as (m') "[CORR MU]".
       rewrite {1}/eo_corr. iDestruct "CORR" as "[CNT ST]".
-      iModIntro. Unshelve. 2: by apply PROD_ENV_INDEP. 
+      iModIntro.
       iSpecialize ("MU" with "[Hf]").
       { iSplitL.
         { iApply has_fuels_proper; [reflexivity| | by iFrame].
-          rewrite insert_union_singleton_l. f_equiv.
+          rewrite insert_union_singleton_l. f_equiv; [reflexivity| ]. 
           erewrite map_fmap_singleton. rewrite insert_empty.
-          f_equiv. apply sub_helper. lia. }
-        set_solver. }
+          f_equiv; [reflexivity| ]. apply sub_helper. lia. }
+        iPureIntro. set_solver. }
       iApply sswp_MU_wp; [done| ]. 
       iApply (wp_store with "[$]"). iIntros "!> CNT".
       iApply (MU_wand with "[-MU] MU").
@@ -244,34 +233,34 @@ Section short_prog.
       (* fold ρEven. *)
 
       (* Set Printing Implicit. *)
-      replace (@inl (amRole (even_AM even_impl) + amRole (odd_AM odd_impl))
-                     _
-                     (even_role (ρ__e even_impl))) with ρEven by done. 
-
+      (* replace (@inl (amRole (even_AM even_impl) + amRole (odd_AM odd_impl)) *)
+      (*                _ *)
+      (*                (even_role (ρ__e even_impl))) with ρEven by done.  *)
       do 2 wp_pure _. 
 
       iApply ("Hg" with "[] [] [-HΦ]"); [..| done]. 
-      3: { iFrame "Hodd_at EVEN Hinv SPLIT HFR". 
+      3: { iFrame "Hodd_at EVEN HFR VS_E VS_O VS_M".
            iApply has_fuels_proper; [reflexivity| | iFrame].
            rewrite insert_empty. erewrite (proj2 (Nat.ltb_ge _ _)); [| lia]. 
            f_equiv; [| f_equiv]. 
            all: apply add_helper; lia. }
       all: iPureIntro; lia.
     - erewrite (proj2 (Nat.ltb_ge _ _)); [| lia].       
-      iPoseProof (odd_vs _ _ _ _ st_res_SR_odd with "[$]") as "#VS".
-      { solve_ndisj. } 
-      rewrite /eo_vs. iMod "VS".
-      iDestruct "VS" as (m') "[CORR MU]".
+      (* iPoseProof (odd_vs _ _ _ _ st_res_SR_odd with "[$]") as "#VS". *)
+      (* { solve_ndisj. }  *)
+      (* rewrite /eo_vs. iMod "VS". *)
+      (* iMod "VS_O" *)
+      iPoseProof "VS_O" as "-#V". iMod "V" as (m') "[CORR MU]".
       rewrite {1}/eo_corr. iDestruct "CORR" as "[CNT ST]".
-      iModIntro. Unshelve. 2: by apply PROD_ENV_INDEP. 
+      iModIntro. 
       iSpecialize ("MU" with "[Hf]").
       { iSplitL.
         { iApply has_fuels_proper; [reflexivity| | by iFrame].
           rewrite insert_commute; [| done]. 
-          rewrite insert_union_singleton_l. f_equiv.
+          rewrite insert_union_singleton_l. f_equiv; [reflexivity| ]. 
           erewrite map_fmap_singleton. rewrite insert_empty.
-          f_equiv. apply sub_helper. lia. }
-        set_solver. }
+          f_equiv; [reflexivity| ]. apply sub_helper. lia. }
+        iPureIntro. set_solver. }
       iApply sswp_MU_wp; [done| ]. 
       iApply (wp_store with "[$]"). iIntros "!> CNT".
       iApply (MU_wand with "[-MU] MU").
@@ -292,30 +281,26 @@ Section short_prog.
 
       simpl. rewrite -insert_union_singleton_l.
       simpl_has_fuels.
-      (* fold ρOdd. *)
-      replace (@inl (amRole (even_AM even_impl) + amRole (odd_AM odd_impl))
-                 _
-                 (odd_role (ρ__o odd_impl))) with ρOdd by done. 
-
       do 2 wp_pure _. 
 
       iApply ("Hg" with "[] [] [-HΦ]"); [..| done]. 
-      3: { iFrame "Heven_at ODD Hinv SPLIT HFR". 
+      3: { iFrame "Heven_at ODD HFR VS_E VS_O VS_M". 
            iApply has_fuels_proper; [reflexivity| | iFrame].
            rewrite insert_commute; [| done].  
            rewrite insert_empty.
            erewrite (proj2 (Nat.ltb_lt _ _)); [| lia]. 
            f_equiv; [| f_equiv]. 
            all: apply add_helper; lia. }
-      all: iPureIntro; lia.      
+      all: iPureIntro; lia.
   Qed.
 
-  Lemma short_spec: even_odd_spec ENV_AM st_res even_at odd_at short.
+  Lemma short_spec: even_odd_spec st_res even_at odd_at st_res_SR_even st_res_SR_odd short.
   Proof using All. 
-    rewrite /even_odd_spec. iIntros (tid n N1 N2 f Hf EVEN). 
-    iIntros (Φ) "(#SPLIT & #INV & Hf & EVEN & ODD & FR) HΦ". unfold short.
-    iApply (short_spec_impl with "[-HΦ]"); [..| done]. 
-    3: { iFrame "EVEN ODD FR SPLIT INV". iApply has_fuels_proper; [reflexivity| | by iFrame].
+    rewrite /even_odd_spec. iIntros (tid n N1 N2 f Hf EVEN ????). 
+    iIntros (Φ) "(#VS_E & #VS_O & #VS_M & Hf & EVEN & ODD & FR) HΦ". unfold short.
+    iApply (short_spec_impl with "[-HΦ]"); try done. 
+    3: { iFrame "EVEN ODD FR VS_E VS_O VS_M". 
+         iApply has_fuels_proper; [reflexivity| | by iFrame].
          erewrite (proj2 (Nat.ltb_lt _ _)); [| lia].
          f_equiv; [| f_equiv].
          all: apply add_helper; lia. }
